src/hmem/trace.lean
@@ -2,37 +2,68 @@ import hmem.memory
 import hmem.split_cost
 import hmem.stack
 
+universe u
+variables {α: Type u} [has_zero α] [decidable_eq α]
+
 namespace hmem
 
 structure trace (α: Type*) [has_zero α] [decidable_eq α] :=
   (result: memory α)
+  (branch: list bool)
   (steps: ℕ)
-  (calls: list (program α × memory α))
-  (recurses: list (memory α)) 
+  (calls: list (memory α))
+  (recurses: list (memory α))
 
-universe u
-variables {α: Type u} [has_zero α] [decidable_eq α]
+def program.calls_on_branch {α: Type*} [has_zero α] [decidable_eq α]:
+  program α → list bool → list (program α)
+| [] _ := []
+| (@instruction.ite _ _ _ _ _ is'::is) (tt::br) := program.calls_on_branch is' br
+| (@instruction.ite _ _ _ _ _ _::is) (ff::br) := program.calls_on_branch is br
+| (instruction.call func _ _::is) br := func :: program.calls_on_branch is br
+| (i::is) br := program.calls_on_branch is br
 
-def trace.has_call_cost (t: trace α) (c: ℕ): Prop :=
-  t.calls.sum_le (λ pm, pm.fst.has_time_cost pm.snd) c
+def trace.prog_calls (t: trace α) (p: program α): list (program α × memory α) :=
+  list.zip (p.calls_on_branch t.branch) t.calls
+
+def trace.has_call_cost (t: trace α) (p: program α) (c: ℕ): Prop :=
+  (t.prog_calls p).sum_le (λ pm, pm.fst.has_time_cost pm.snd) c
   
 def trace.has_recurse_cost (t: trace α) (p: program α) (r: ℕ): Prop :=
   t.recurses.sum_le (λ m, p.has_time_cost m) r
 
+def thunk.extend_branch (tr: thunk α) (br: list bool): list bool :=
+  match tr.takes_branch with
+  | (some b) := b::br
+  | none := br
+  end
+
 def thunk.extend_trace (t: thunk α): trace α → trace α
-| ⟨m, i, cs, rs⟩ := match t.step with
-  | (sum.inr (sum.inr (option.some p, m', _))) := ⟨m, i + 1, (p, m')::cs, rs⟩
-  | (sum.inr (sum.inr (option.none, m', _))) := ⟨m, i + 1, cs, m'::rs⟩
-  | _ := ⟨m, i + 1, cs, rs⟩
+| ⟨m, br, i, cs, rs⟩ := match t.step with
+  | (sum.inr (sum.inr (option.some p, m', _))) := ⟨m, br, i + 1, m'::cs, rs⟩
+  | (sum.inr (sum.inr (option.none, m', _))) := ⟨m, br, i + 1, cs, m'::rs⟩
+  | _ := ⟨m, t.extend_branch br, i + 1, cs, rs⟩
 end
 
-def thunk.extend_trace₀ {t t': thunk α} {tr: trace α} {m: memory α} {n: ℕ} {cs: list (program α × memory α)} {rs: list (memory α)}:
-  t.step = sum.inl t' → tr = ⟨m, n, cs, rs⟩ → t.extend_trace tr = ⟨m, n+1, cs, rs⟩ :=
+def thunk.extend_trace₀ {t t': thunk α} {tr: trace α} {m: memory α} {br: list bool} {n: ℕ} {cs: list (memory α)} {rs: list (memory α)}:
+  t.step = sum.inl t' → tr = ⟨m, br, n, cs, rs⟩ → t.takes_branch = none → t.extend_trace tr = ⟨m, br, n+1, cs, rs⟩ :=
 begin
   intros hstep heq,
-  simp only [heq, thunk.extend_trace, hstep, eq_self_iff_true, and_true],
+  simp only [heq, thunk.extend_trace, thunk.extend_branch, hstep, eq_self_iff_true, and_true, true_and],
+  intro h,
+  rw [h],
+  trivial,
 end
-  
+
+
+def thunk.extend_trace_if {t t': thunk α} {tr: trace α} {m: memory α} {b: bool} {br: list bool} {n: ℕ} {cs: list (memory α)} {rs: list (memory α)}:
+  t.step = sum.inl t' → tr = ⟨m, br, n, cs, rs⟩ → t.takes_branch = some b → t.extend_trace tr = ⟨m, b::br, n+1, cs, rs⟩ :=
+begin
+  intros hstep heq,
+  simp only [heq, thunk.extend_trace, thunk.extend_branch, hstep, eq_self_iff_true, and_true, true_and],
+  intro h,
+  rw [h],
+  trivial,
+end
 
 theorem thunk.extend_trace_result (t : thunk α) (tr: trace α):
   (t.extend_trace tr).result = tr.result :=
@@ -61,11 +92,11 @@ begin
 end
 
 theorem thunk.extend_trace_calls_cons {t: thunk α} {tr: trace α} {p: program α} {t': thunk α × list α} {m: memory α}:
-  t.step = sum.inr (sum.inr (some p, m, t')) → (t.extend_trace tr).calls = (p, m)::tr.calls :=
+  t.step = sum.inr (sum.inr (some p, m, t')) → (t.extend_trace tr).calls = m::tr.calls :=
 begin
   cases tr,
   intro hstep,
-  simp only [thunk.extend_trace, hstep, eq_self_iff_true, and_true]
+  simp only [thunk.extend_trace, hstep, eq_self_iff_true, and_true],
 end
 
 theorem thunk.extend_trace_calls_eq {t: thunk α} {tr: trace α}:
@@ -152,12 +183,12 @@ begin
 end
 
 inductive thunk.has_trace: thunk α → trace α → Prop
-| result (p: program α) (m: memory α): thunk.has_trace ⟨p, [], m⟩ ⟨m, 0, [], []⟩
+| result (p: program α) (m: memory α): thunk.has_trace ⟨p, [], m⟩ ⟨m, [],  0, [], []⟩
 | step {t t': thunk α} {tr: trace α} (ht: t.step_over t') (htr: thunk.has_trace t' tr):
   thunk.has_trace t (thunk.extend_trace t tr)
 
 theorem thunk.has_trace_nil (t: thunk α) {tr: trace α}:
-  t.has_trace tr → t.current = [] → tr = ⟨t.state, 0, [], []⟩ :=
+  t.has_trace tr → t.current = [] → tr = ⟨t.state, [], 0, [], []⟩ :=
 begin
   intros htr ht,
   cases htr,
@@ -176,23 +207,131 @@ begin
   exact ⟨_, htr_ht, htr_ih⟩
 end
 
+
+theorem trace.extend_prog_calls_eq {t t': thunk α} (tr: trace α) (htr: t'.has_trace tr):
+  (∀ {p x}, t.step ≠ sum.inr (sum.inr (some p, x))) →
+  t.step_over t' →
+  (t.extend_trace tr).prog_calls t.current = tr.prog_calls t'.current :=
+begin
+  intros hstep hso,
+  cases tr,
+  cases t,
+  cases t_current,
+  { simpa only [thunk.step_over, thunk.step] using hso },
+  cases t_current_hd;
+  try {
+    simp only [thunk.step_over, thunk.step] at hso,
+    simp only [thunk.step, program.calls_on_branch, thunk.takes_branch, trace.prog_calls, trace.calls, thunk.extend_trace, thunk.extend_branch, ← hso] },
+  { split_ifs;
+    simp only [thunk.extend_branch, program.calls_on_branch] },
+  { contrapose! hstep,
+    simp only [thunk.step, sum.inr.inj_iff, prod.mk.inj_iff, exists_eq_right', exists_eq'] },
+  rw [hso.right],
+  refl,
+end
+
+theorem trace.extend_prog_calls_eq₀ {t t': thunk α} (tr: trace α) (htr: t'.has_trace tr):
+  t.step = sum.inl t' →
+  (t.extend_trace tr).prog_calls t.current = tr.prog_calls t'.current :=
+begin
+  intro h,
+  apply trace.extend_prog_calls_eq,
+  exact htr,
+  exact λ _ _, h.symm ▸ sum.inl_ne_inr,
+  simp only [thunk.step_over, h],
+end
+
+theorem trace.extend_prog_calls_eq₁ {t: thunk α} (tr: trace α) (m: memory α) (htr: t.has_trace tr):
+  t.step = sum.inr (sum.inl m) →
+  (t.extend_trace tr).prog_calls t.current = tr.prog_calls t.current :=
+begin
+  intro hstep,
+  cases tr,
+  cases t,
+  cases t_current,
+  { simp only [thunk.extend_trace, hstep, trace.prog_calls, thunk.extend_branch, thunk.takes_branch] },
+  cases t_current_hd;
+  simpa [thunk.step] using hstep,
+end
+
+theorem trace.extend_prog_calls_eq₂ {t t' t'': thunk α} (tr: trace α) (r) (m: memory α) (htr: t'.has_trace tr):
+  t.step = sum.inr (sum.inr (none, m, t'', r)) →
+  t.step_over t' →
+  (t.extend_trace tr).prog_calls t.current = tr.prog_calls t'.current :=
+begin
+  intros hstep hso,
+  apply trace.extend_prog_calls_eq,
+  exact htr,
+  { intros _ _,
+    simpa only [hstep, ← push_neg.not_eq, prod.mk.inj_iff, false_and] using not_false },
+  exact hso
+end
+
+theorem trace.extend_prog_calls_cons {t t': thunk α} (tr: trace α) {p: program α} {m: memory α} (htr: t'.has_trace tr) {r: list α}:
+  t.step = sum.inr (sum.inr (some p, m, t', r)) →
+  (t.extend_trace tr).prog_calls t.current = (p, m) :: tr.prog_calls t'.current :=
+begin
+  intro hstep,
+  cases tr,
+  simp only [hstep, thunk.extend_trace, trace.prog_calls,
+    program.calls_on_branch],
+  cases t,
+  cases t_current,
+  simpa only [thunk.step] using hstep,
+  cases t_current_hd;
+  try { simpa only [thunk.step, prod.mk.inj_iff, false_and] using hstep };
+  simp only [thunk.step, prod.mk.inj_iff] at hstep,
+  simpa only [program.calls_on_branch, thunk.takes_branch, thunk.extend_branch, ← hstep]
+    using list.zip_cons_cons _ _ _ _,
+end
+
+theorem trace.extend_prog_calls_cons' {t t' t'': thunk α} (tr: trace α) {p: program α} {m: memory α} (htr: t''.has_trace tr) {r: list α}:
+  t.step = sum.inr (sum.inr (some p, m, t', r)) →
+  t'.current = t''.current →
+  (t.extend_trace tr).prog_calls t.current = (p, m) :: tr.prog_calls t''.current :=
+begin
+  intros hstep heq,
+  cases tr,
+  simp only [hstep, thunk.extend_trace, trace.prog_calls,
+    program.calls_on_branch],
+  cases t,
+  cases t_current,
+  simpa only [thunk.step] using hstep,
+  cases t_current_hd;
+  try { simpa only [thunk.step, prod.mk.inj_iff, false_and] using hstep };
+  simp only [thunk.step, prod.mk.inj_iff] at hstep,
+  simpa only [program.calls_on_branch, thunk.takes_branch, thunk.extend_branch, ← hstep, ← heq]
+    using list.zip_cons_cons _ _ _ _,
+end
+
 theorem thunk.has_trace.exists_calls_sum {t: thunk α} {tr: trace α}:
-  t.has_trace tr → ∃ c, tr.has_call_cost c :=
+  t.has_trace tr → ∃ c, tr.has_call_cost t.current c :=
 begin
   unfold trace.has_call_cost,
   intro htr,
   induction htr,
-  { exact ⟨0, trivial⟩ },
+  { refine ⟨0, _⟩,
+    unfold trace.prog_calls trace.calls,
+    rw [list.zip_nil_right],
+    trivial },
   cases hstep:htr_t.step,
-  { rwa [thunk.extend_trace_calls_eq₀ hstep] },
+  { simp only [thunk.step_over, hstep] at htr_ht,
+    rwa [trace.extend_prog_calls_eq₀ _ _ hstep, htr_ht],
+    rwa [htr_ht], },
   cases val,
-  { rwa [thunk.extend_trace_calls_eq₁ hstep] },
-  rcases val with ⟨_|_, _, _⟩,
-  { rwa [thunk.extend_trace_calls_eq₂ hstep] },
+  { simpa only [thunk.step_over, hstep] using htr_ht },
+  rcases val with ⟨_|_, _, _, _⟩,
+  { rwa [trace.extend_prog_calls_eq₂ _ _ _ _ hstep],
+    exact htr_ht,
+    exact htr_htr },
   { simp only [thunk.step_over, option.get_or_else, option.map_some', hstep] at htr_ht,
     cases htr_ht.left with c₀ hc₀,
-    cases htr_ih with c₁ hc₁,rw [thunk.extend_trace_calls_cons hstep],
-    exact ⟨_, _, _, ⟨_, hc₀⟩, hc₁, rfl⟩ }
+    cases htr_ih with c₁ hc₁,
+    rw [trace.extend_prog_calls_cons' _ _ hstep],
+    refine ⟨_, c₀, c₁, ⟨_, hc₀⟩, hc₁, rfl⟩,
+    apply thunk.set_result_current htr_ht.right.symm,
+    apply htr_htr,
+  }
 end
 
 theorem thunk.has_trace.exists_recurses_sum {t: thunk α} {tr: trace α}:
@@ -218,7 +357,7 @@ end
 
 theorem thunk.has_trace.split_cost {t: thunk α} {tr: trace α} {c r: ℕ}:
   t.has_trace tr →
-  tr.has_call_cost c →
+  tr.has_call_cost t.current c →
   tr.has_recurse_cost t.function r →
   t.split_time_cost (tr.steps + 1) c r :=
 begin
@@ -227,26 +366,36 @@ begin
   induction htr generalizing c r,
   { exact λ _ _, or.inl rfl },
   cases hstep:htr_t.step,
-  { rw [thunk.extend_trace_calls_eq₀ hstep, thunk.extend_trace_recurses_eq₀ hstep, thunk.extend_trace_steps, thunk.step_over_function htr_ht],
+  { rw [trace.extend_prog_calls_eq₀ _ _ hstep, thunk.extend_trace_recurses_eq₀ hstep, thunk.extend_trace_steps, thunk.step_over_function htr_ht],
     intros hcs hrs,
     refine or.inr ⟨_, _, _, _, _, _, htr_ht, _, (zero_add _).symm, (zero_add _).symm⟩,
     { simp only [thunk.external_time_cost_step, hstep] },
-    exact htr_ih hcs hrs },
+    simp only [thunk.step_over, hstep] at htr_ht,
+    rw [htr_ht] at hcs,
+    exact htr_ih hcs hrs,
+    simp only [thunk.step_over, hstep] at htr_ht,
+    rw [htr_ht],
+    apply htr_htr },
   cases val,
   { simpa only [thunk.step_over, thunk.step, hstep] using htr_ht },
-  rcases val with ⟨_ | _, _, _⟩,
-  { rw [thunk.extend_trace_calls_eq₂ hstep, thunk.extend_trace_recurses_cons hstep, thunk.extend_trace_steps, thunk.step_over_function htr_ht],
+  rcases val with ⟨_ | _, _, _, _⟩,
+  { rw [trace.extend_prog_calls_eq₂ _ _ _ _ hstep, thunk.extend_trace_recurses_cons hstep, thunk.extend_trace_steps, thunk.step_over_function htr_ht],
     intros hcs hrs,
     rcases hrs with ⟨r₀, r₁, hrcost, hrs, hr⟩,
     refine or.inr ⟨_, _, _, _, _, _, htr_ht, _, (zero_add _).symm, hr⟩,
     { simpa only [thunk.external_time_cost_step, hstep, option.map_none', option.get_or_else, thunk.step_over_function htr_ht] using hrcost },
-    exact htr_ih hcs hrs },
-  { rw [thunk.extend_trace_calls_cons hstep, thunk.extend_trace_recurses_eq₂ hstep, thunk.extend_trace_steps, thunk.step_over_function htr_ht],
+    exact htr_ih hcs hrs,
+    exact htr_ht,
+    exact htr_htr, },
+  { rw [trace.extend_prog_calls_cons' _ _ hstep, thunk.extend_trace_recurses_eq₂ hstep, thunk.extend_trace_steps, thunk.step_over_function htr_ht],
     intros hcs hrs,
     rcases hcs with ⟨c₀, c₁, hccost, hcs, hc⟩,
     refine or.inr ⟨_, _, _, _, _, _, htr_ht, _, hc, (zero_add _).symm⟩,
     { simpa only [thunk.external_time_cost_step, hstep, option.map_some', option.get_or_else] using hccost },
-    exact htr_ih hcs hrs },
+    exact htr_ih hcs hrs,
+    simp only [thunk.step_over, hstep] at htr_ht,
+    apply thunk.set_result_current htr_ht.right.symm,
+    apply htr_htr },
 end
 
 def program.has_trace (p: program α) (m: memory α) (t: trace α): Prop := thunk.has_trace ⟨p, p, m⟩ t
@@ -266,7 +415,7 @@ end
 
 theorem program.has_trace.call_cost {p: program α} {m: memory α} {tr: trace α} {c: ℕ}:
   p.has_trace m tr →
-  tr.has_call_cost c →
+  tr.has_call_cost p c →
   p.call_cost m c :=
 begin
   intros htr hc,
@@ -297,12 +446,33 @@ theorem step_trace {t t': thunk α} {tr tr': trace α}:
   t.has_trace tr :=
 λ hso hex htr, hex ▸ thunk.has_trace.step hso htr
 
+theorem if_true_trace {r: memory α} {p: program α} {m: memory α} {n cn: ℕ} {cond: vector α cn → Prop} [Π {v}, decidable (cond v)] {src: vector (source α) cn} {br: list bool} {is is': program α} {cs rs: list (memory α)}:
+  cond (src.map (λ s, m.getvs s)) →
+  thunk.has_trace ⟨p, is', m⟩ ⟨r, br, n, cs, rs⟩ →
+  thunk.has_trace ⟨p, (instruction.ite cond src is')::is, m⟩ ⟨r, tt::br, n+1, cs, rs⟩ :=
+begin
+  intros hcond htr,
+  apply step_trace _ _ htr,
+  { simp only [thunk.step_over, thunk.step, hcond, if_true, eq_self_iff_true, and_true] },
+  simp only [thunk.extend_trace, thunk.step, thunk.extend_branch, thunk.takes_branch, hcond, if_true, eq_self_iff_true, and_true, true_and],
+end
 
-theorem call_trace {pc: program α} {d s: source α} {p is: program α} {m m' mr r: memory α} {n: ℕ} {cs: list (program α × memory α)} {rs: list (memory α)}:
+theorem if_false_trace {r: memory α} {p: program α} {m: memory α} {n cn: ℕ} {cond: vector α cn → Prop} [Π {v}, decidable (cond v)] {src: vector (source α) cn} {br: list bool} {is is': program α} {cs rs: list (memory α)}:
+  ¬ cond (src.map (λ s, m.getvs s)) →
+  thunk.has_trace ⟨p, is, m⟩ ⟨r, br, n, cs, rs⟩ →
+  thunk.has_trace ⟨p, (instruction.ite cond src is')::is, m⟩ ⟨r, ff::br, n+1, cs, rs⟩ :=
+begin
+  intros hcond htr,
+  apply step_trace _ _ htr,
+  { simp only [thunk.step_over, thunk.step, hcond, if_false, eq_self_iff_true, and_true] },
+  simp only [thunk.extend_trace, thunk.step, thunk.extend_branch, thunk.takes_branch, hcond, if_false, eq_self_iff_true, and_true, true_and],
+end
+
+theorem call_trace {pc: program α} {d s: source α} {p is: program α} {m m' mr r: memory α} {br: list bool} {n: ℕ} {cs rs: list (memory α)}:
   m.getms s = m' →
   pc.has_result m' mr →
-  thunk.has_trace ⟨p, is, m.setmp (d.get m) mr⟩ ⟨r, n, cs, rs⟩ →
-  thunk.has_trace ⟨p, (instruction.call pc d s)::is, m⟩ ⟨r, n+1, (pc,m')::cs, rs⟩ :=
+  thunk.has_trace ⟨p, is, m.setmp (d.get m) mr⟩ ⟨r, br, n, cs, rs⟩ →
+  thunk.has_trace ⟨p, (instruction.call pc d s)::is, m⟩ ⟨r, br, n+1, m'::cs, rs⟩ :=
 begin
   intros hm hres htr,
   apply step_trace _ _ htr,
@@ -314,11 +484,11 @@ begin
     rw [hm] }
 end
 
-theorem recurse_trace {p: program α} {d s: source α} {is: program α} {m m' mr r: memory α} {n: ℕ} {cs: list (program α × memory α)} {rs: list (memory α)}:
+theorem recurse_trace {p: program α} {d s: source α} {is: program α} {m m' mr r: memory α} {br: list bool} {n: ℕ} {cs rs: list (memory α)}:
   m.getms s = m' →
   p.has_result m' mr →
-  thunk.has_trace ⟨p, is, m.setmp (d.get m) mr⟩ ⟨r, n, cs, rs⟩ →
-  thunk.has_trace ⟨p, (instruction.recurse d s)::is, m⟩ ⟨r, n+1, cs, m'::rs⟩ :=
+  thunk.has_trace ⟨p, is, m.setmp (d.get m) mr⟩ ⟨r, br, n, cs, rs⟩ →
+  thunk.has_trace ⟨p, (instruction.recurse d s)::is, m⟩ ⟨r, br, n+1, cs, m'::rs⟩ :=
 begin
   intros hm hres htr,
   apply step_trace _ _ htr,
@@ -331,6 +501,6 @@ begin
 end
 
 theorem end_trace {p: program α} {m m': memory α}:
-  m = m' → thunk.has_trace ⟨p, [], m⟩ ⟨m', 0, [], []⟩ := λ h, h ▸ thunk.has_trace.result p m
+  m = m' → thunk.has_trace ⟨p, [], m⟩ ⟨m', [], 0, [], []⟩ := λ h, h ▸ thunk.has_trace.result p m
 
 end hmem
